wip

DY/Label/Basic.lean
@@ -4,12 +4,70 @@ public import DY.Trace.Basic
 
 namespace DY
 
-variable [BytesFunctor]
+variable [ExecTraceTypes]
 
 public
-structure Label where
-  isCorrupt_: Trace Unit → Prop
-  isCorruptSnoc_:
-    ∀ tr e, isCorrupt_ tr → isCorrupt_ (.snoc tr e)
+structure Label [ExecTraceTypes] where
+  isCorrupt: ExecTrace → Prop
+  isCorruptLater:
+    ∀ tr1 tr2, tr1 ≤ tr2 → isCorrupt tr1 → isCorrupt tr2
+    := by grind
+
+@[scoped grind→]
+public
+theorem _root_.DY.Trace.MonotoneLemmas.isCorruptLater (l: Label) (tr1 tr2: ExecTrace):
+  tr1 ≤ tr2 →
+  l.isCorrupt tr1 →
+  l.isCorrupt tr2
+  := by
+    exact l.isCorruptLater tr1 tr2
+
+@[ext]
+public
+theorem Label.ext
+  [ExecTraceTypes]
+  (l1 l2: Label)
+  : (∀ tr: ExecTrace, l1.isCorrupt tr = l2.isCorrupt tr) →
+  l1 = l2
+  := by
+    cases l1
+    cases l2
+    simp
+    grind
+
+@[expose]
+public
+def Label.canFlow (l1: Label) (l2: Label) (tr: ExecTrace): Prop :=
+  ∀ trLater,
+    tr ≤ trLater →
+    l2.isCorrupt trLater → l1.isCorrupt trLater
+
+@[scoped grind→]
+public
+theorem _root_.DY.Trace.MonotoneLemmas.canFlowLater (l1: Label) (l2: Label) (tr1 tr2: ExecTrace):
+  tr1 ≤ tr2 →
+  l1.canFlow l2 tr1 →
+  l1.canFlow l2 tr2
+  := by
+    unfold Label.canFlow
+    grind [Trace.le_trans]
+
+@[grind]
+public
+theorem canFlowRefl (l: Label) (tr: ExecTrace):
+  l.canFlow l tr
+  := by
+    unfold Label.canFlow
+    grind
+
+-- @[grind]
+public
+theorem canFlowTrans (l1: Label) (l2: Label) (l3: Label) (tr: ExecTrace):
+  l1.canFlow l2 tr →
+  l2.canFlow l3 tr →
+  l1.canFlow l3 tr
+  := by
+    unfold Label.canFlow
+    grind
 
 end DY
