DY/Trace.lean
@@ -1,4 +1,5 @@
 module
 
 public import DY.Trace.Basic
+public import DY.Trace.Invariant
 public import DY.Trace.Manipulation
