DY/Trace/AttackerKnowledge.lean
@@ -1,0 +1,12 @@
+import DY.Bytes.Basic
+import DY.Trace.Basic
+
+namespace DY
+
+structure ExecEntryAttackerKnowledge [BytesFunctor] [ExecTraceTypes] (ExecEntryT: ExecEntryType) where
+  attackerKnows: ExecTrace → ExecEntryT.type → Bytes → Prop
+
+class ExecTraceAttackerKnowledge [BytesFunctor] [ExecTraceTypes] where
+  attackerKnows: ∀ id, ExecEntryAttackerKnowledge (ExecTraceTypes.entries id)
+
+end DY
