DY/Trace/Invariant.lean
@@ -1,0 +1,97 @@
+module
+
+public import DY.Trace.Basic
+
+namespace DY
+
+public
+structure ProofEntryType (ExecEntryT: ExecEntryType) where
+  type: [ExecTraceTypes] → Type
+  erase: ∀ [ExecTraceTypes], type → ExecEntryT.type
+
+public
+class ProofTraceTypes [ExecTraceTypes] where
+  proofEntries: ∀ id, ProofEntryType (ExecTraceTypes.entries id)
+
+public
+class abbrev TraceTypes := ExecTraceTypes, ProofTraceTypes
+
+public
+structure ProofTrace.Entry [TraceTypes] where
+  id: Fin ExecTraceTypes.n
+  entry: (ProofTraceTypes.proofEntries id).type
+
+public
+abbrev ProofTrace [TraceTypes] := Trace ProofTrace.Entry
+
+public
+def ProofTrace.Entry.erase
+  [TraceTypes]
+  (entry: ProofTrace.Entry)
+  : ExecTrace.Entry
+where
+  id := entry.id
+  entry := (ProofTraceTypes.proofEntries entry.id).erase entry.entry
+
+public
+def Trace.erase
+  [TraceTypes]
+  (tr: ProofTrace)
+  : ExecTrace
+:=
+  match tr with
+  | .nil => .nil
+  | .snoc trBefore entry => .snoc trBefore.erase entry.erase
+
+public
+theorem Trace.erase_le [TraceTypes] (tr1 tr2: ProofTrace)
+  : tr1 ≤ tr2 →
+    tr1.erase ≤ tr2.erase
+:= by
+  intro h_le
+  induction h_le
+  · apply Trace.le.equal
+  · apply Trace.le.extend
+    assumption
+
+grind_pattern Trace.erase_le => tr1 ≤ tr2, tr1.erase
+
+-- public
+-- theorem Trace.erase_append
+--   [TraceTypes]
+--   (tr: ProofTrace) (entry: ProofTrace.Entry)
+--   : (tr.append entry).erase = tr.erase.append entry.erase
+-- := by
+--   rfl
+
+-- TODO test coercion
+example [TraceTypes]: Coe ProofTrace ExecTrace where
+  coe tr := tr.erase
+
+-- Invariant
+
+public
+structure ProofTraceEntryInvariant
+  [TraceTypes]
+  {ExecEntryT: ExecEntryType}
+  (ProofEntryT: ProofEntryType ExecEntryT)
+where
+  invariant: ProofTrace → ProofEntryT.type → Prop
+
+public
+class ProofTraceInvariants [TraceTypes] where
+  invariants: ∀ id, ProofTraceEntryInvariant (ProofTraceTypes.proofEntries id)
+
+public
+def Trace.Invariant
+  [TraceTypes] [ProofTraceInvariants]
+  (tr: ProofTrace)
+  : Prop
+:=
+  match tr with
+  | .nil => True
+  | .snoc trBefore entry =>
+    trBefore.Invariant ∧
+    (ProofTraceInvariants.invariants entry.id).invariant trBefore entry.entry
+
+end DY
